Added test13 target with Antoine. WIP in Record.fst and TLS.fst

src/tls/Record.fst
@@ -12,7 +12,9 @@ open TLSConstants
 open Range
 open Content
 
-// Consider merging this module with Content?
+
+
+// Consider merging some of this module with Content?
 
 // ------------------------outer packet format -------------------------------
 
@@ -31,7 +33,10 @@ let makePacket ct ver (data: b:bytes { repr_bytes (length b) <= 2}) =
    @| bytes_of_int 2 (length data) 
    @| data 
 
-val parseHeader: h5:header -> Tot (result (contentType * protocolVersion * int))
+
+val parseHeader: h5:header -> Tot (result (contentType 
+                                         * protocolVersion 
+                                         * l:nat { l <= max_TLSCiphertext_fragment_length}))
 let parseHeader (h5:header) =
     let (ct1,b4)   = Platform.Bytes.split h5 1 in
     let (pv2,len2) = Platform.Bytes.split b4 2 in
@@ -63,6 +68,53 @@ let recordPacketOut (i: AEAD_GCM.gid) (wr:StatefulLHAE.writer i) (pv: protocolVe
         StatefulLHAE.encrypt #i #ad #rg wr f
     in
     makePacket ct pv payload
+
+
+(*** networking (floating) ***)
+
+effect EXT (a:Type) = ST a
+  (requires (fun _ -> True)) 
+  (ensures (fun h0 _ h1 -> modifies Set.empty h0 h1))
+
+//16-05-19  to be patched in ulib
+val tcp_recv: Platform.Tcp.networkStream -> max:nat -> EXT (optResult string (b:bytes {length b <= max}))
+let tcp_recv = assume false; Platform.Tcp.recv
+
+
+private val really_read_rec: b:bytes -> Platform.Tcp.networkStream -> l:nat -> EXT (result (lbytes (l+length b)))
+
+let rec really_read_rec prev tcp len = 
+    if len = 0 
+    then Correct prev
+    else 
+      match Platform.Tcp.recv tcp len with
+      | Correct b -> 
+            let lb = length b in
+      	    if lb = len then Correct(prev @| b)
+      	    else really_read_rec (prev @| b) tcp (len - lb)
+      | Error e -> Error(AD_internal_error,e)
+
+private let really_read = really_read_rec empty_bytes
+
+val read: Platform.Tcp.networkStream -> protocolVersion -> 
+  EXT (result (contentType * protocolVersion * b:bytes { length b <= max_TLSCiphertext_fragment_length}))
+
+// in the spirit of TLS 1.3, we ignore the outer protocol version (see appendix C):
+// our server never treats the ClientHello's record pv as its minimum supported pv;
+// our client never checks the consistency of the server's record pv.
+// (see earlier versions for the checks we used to perform)
+
+let read tcp pv =
+  match really_read tcp 5 with 
+  | Correct header -> (
+      match parseHeader header with  
+      | Correct (ct,pv,len) -> (
+         match really_read tcp len with
+         | Correct payload  -> Correct (ct,pv,payload)
+         | Error e          -> Error e )
+      | Error e             -> Error e )
+  | Error e                 -> Error e
+
 
 (* TODO
 let recordPacketIn i (rd:StatefulLHAE.reader i) ct payload =
